Theorem from uniform bytes spec (#455)
* - Add function split64to32 that given an array of 64 bytes split it into two
  arrays of 32 bytes.

Curve25519Dalek/Specs/Ristretto/RistrettoPoint/FromUniformBytes.lean
@@ -5,6 +5,7 @@ Authors: Markus Dablander
 -/
 import Curve25519Dalek.Funs
 import Curve25519Dalek.Defs.Edwards.Representation
+import Curve25519Dalek.Specs.Backend.Serial.U64.Field.FieldElement51.FromBytes
 
 /-! # Spec Theorem for `RistrettoPoint::from_uniform_bytes`
 
@@ -20,7 +21,8 @@ and adding the resulting two Ristretto points via elliptic curve addition.
 - Complete proof
 -/
 
-open Aeneas.Std Result
+open Aeneas.Std Result core.ops.range
+
 namespace curve25519_dalek.ristretto.RistrettoPoint
 
 /-
@@ -51,11 +53,59 @@ natural language specs:
 - The output is a mathematically valid Ristretto point
 -/
 
+def split64to32 (input : Array U8 64#usize) : Result (Array U8 32#usize × Array U8 32#usize) :=
+  let a1 := input.subslice (Range.mk 0#usize 32#usize)
+  let a2 := input.subslice (Range.mk 32#usize 64#usize)
+  match a1, a2 with
+  | ok s1, ok s2 => ok (Array.from_slice (Array.repeat 32#usize 0#u8) s1,
+                        Array.from_slice (Array.repeat 32#usize 0#u8) s2)
+  | _, _ => fail Error.panic
+
+@[progress]
+theorem split64to32_spec (input : Array U8 64#usize) :
+    ∃ a1 a2,
+        split64to32 input = ok (a1, a2) ∧
+        (∀ i : ℕ, i < 32 → a1.val[i]! = input.val[i]! ∧ a2.val[i]! = input.val[i + 32]!) := by
+  simp [split64to32]
+  have h1 :=
+    Array.subslice_spec input (Range.mk 0#usize 32#usize)
+      (by scalar_tac) (by scalar_tac)
+  have h2 :=
+    Array.subslice_spec input (Range.mk 32#usize 64#usize)
+      (by scalar_tac) (by scalar_tac)
+  rcases h1 with ⟨s1, ha1, hs1, hget1⟩
+  rcases h2 with ⟨s2, ha2, hs2, hget2⟩
+  refine ⟨
+    Array.from_slice (Array.repeat 32#usize 0#u8) s1,
+    Array.from_slice (Array.repeat 32#usize 0#u8) s2,
+    ?_, ?_
+  ⟩
+  · simp [ha1, ha2]
+  · intro i hi
+    simp [Array.from_slice]
+    have hsl1 : ↑s1.length = 32 := by scalar_tac
+    have hsl2 : ↑s2.length = 32 := by scalar_tac
+    constructor
+    · simp only [Slice.length] at hsl1
+      simp [hsl1]
+      simp_all only [UScalar.ofNat_val_eq, List.slice_zero_j, add_zero, List.length_take, List.Vector.length_val,
+        Nat.reduceLeDiff, inf_of_le_left, getElem!_pos, List.getElem_take, zero_add, List.getElem!_eq_getElem?_getD,
+        Slice.length, getElem?_pos, Option.getD_some]
+    · simp only [Slice.length] at hsl2
+      simp [hsl2]
+      simp_all only [UScalar.ofNat_val_eq, add_zero, List.length_take, List.getElem_take, zero_add,
+      List.getElem!_eq_getElem?_getD, Slice.length, getElem?_pos, Option.getD_some, List.slice, Nat.reduceSub,
+      List.getElem_take, List.getElem_drop, Nat.add_comm 32 i]
+      grind only [= List.getElem_drop, = List.getElem?_drop, → List.getElem_of_getElem?,
+        = Option.getD_some, = List.getElem?_eq_none, = List.length_take, = getElem?_pos,
+        = getElem?_neg, = min_def, = List.drop_zero, = List.length_drop, = Nat.min_def,
+        = List.getElem?_take]
+
 @[progress]
 theorem from_uniform_bytes_spec (bytes : Array U8 64#usize) :
     ∃ rist,
-    from_uniform_bytes bytes = ok rist ∧
-    rist.IsValid := by
-    sorry
+      from_uniform_bytes bytes = ok rist ∧
+      rist.IsValid := by
+  sorry
 
 end curve25519_dalek.ristretto.RistrettoPoint
